WIP: first draft of specification of the switcher

theories/examples/switcher/switcher_spec.v
@@ -6,12 +6,86 @@ From cap_machine Require Import switcher.
 
 Section Switcher.
   Context
-    {Σ : gFunctors}
-      {ceriseg: ceriseG Σ}
-      {sealsg: sealStoreG Σ}
-      {nainv: logrel_na_invs Σ}
-      {MP: MachineParameters}
-  .
+    {Σ:gFunctors}
+    {ceriseg:ceriseG Σ} {sealsg: sealStoreG Σ}
+    {Cname : CmptNameG}
+    {stsg : STSG Addr region_type Σ} {heapg : heapGS Σ}
+    {nainv: logrel_na_invs Σ}
+    `{MP: MachineParameters}.
+
+  Notation STS := (leibnizO (STS_states * STS_rels)).
+  Notation STS_STD := (leibnizO (STS_std_states Addr region_type)).
+  Notation CVIEW := (prodO STS_STD STS).
+  Notation WORLD := (gmapO CmptName CVIEW).
+  Implicit Types WC : CVIEW.
+  Implicit Types W : WORLD.
+  Implicit Types C : CmptName.
+
+  (* TODO should depend on the number of registers used by entry point. *)
+  Definition is_arg_rmap (rmap : Reg) :=
+    dom rmap = {[ ca0 ; ca1 ; ca2 ; ca3 ; ca4 ; ca5 ; ca5 ; ct0 ]}.
+
+  (* TODO:
+     - How do we treat our own stack frame?
+       I think the ideas is that, we can just to frame it.
+     - What are the constraints about w_entry_point?
+       I think we just want it to be safe-to-share for
+       private transitions of the world.
+     - How to encode the number of registers to pass as arguments?
+       A possibility is to use a resource that encodes it.
+     - Where is the code? Where is MTDC and trusted stack?
+       We need to have a switcher state invariant.
+   *)
+  Lemma switcher_cc_specification
+    (E : coPset)
+    (W0 W1 : WORLD)
+    (C : CmptName)
+    (g_switcher : Locality)
+    (b_switcher e_switcher a_switcher_cc : Addr)
+    (b_stk e_stk a_stk : Addr)
+    (ot_switcher : OType)
+    (wcgp_caller wcra_caller : Word)
+    (w_entry_point : Word)
+    (stk_mem : list Word)
+    (arg_rmap rmap : Reg)
+    (φ : val -> iPropI Σ) :
+
+    is_arg_rmap arg_rmap ->
+    dom rmap = all_registers_s ∖ ((dom arg_rmap) ∪ {[ PC ; cgp ; cra ; csp ; cs0 ]} ) ->
+    (
+      PC ↦ᵣ WCap XSRW_ g_switcher b_switcher e_switcher a_switcher_cc
+      ∗ cgp ↦ᵣ wcgp_caller
+      ∗ cra ↦ᵣ wcra_caller
+      ∗ csp ↦ᵣ WCap RWL Local b_stk e_stk a_stk
+      ∗ cs0 ↦ᵣ w_entry_point (* TODO what to write here exactly? *)
+      ∗ ( [∗ map] rarg↦warg ∈ arg_rmap, rarg ↦ᵣ warg ∗ interp W1 C warg )
+      ∗ ( [∗ map] r↦w ∈ rmap, r ↦ᵣ w )
+
+      ∗ [[ a_stk , e_stk ]] ↦ₐ [[ stk_mem ]]
+
+      ∗ region W0 C ∗ sts_full_world W0 C
+
+      ∗ ( [[ a_stk , e_stk ]] ↦ₐ [[ region_addrs_zeroes a_stk e_stk ]]
+          ∗ region W0 C ∗ sts_full_world W0 C
+          -∗ region W1 C ∗ sts_full_world W1 C)
+      ∗ ▷ ( ∃ (W2 : WORLD) (rmap' : Reg),
+              ⌜ related_sts_pub_world W1 W2 C ⌝
+              ∗ ⌜ dom rmap' = all_registers_s ∖ {[ PC ; cgp ; cra ; csp ; ca0 ; ca1 ]} ⌝
+              ∗ region W2 C ∗ sts_full_world W2 C
+              ∗ PC ↦ᵣ updatePcPerm wcra_caller
+              ∗ cgp ↦ᵣ wcgp_caller ∗ (∃ wret, cra ↦ᵣ wret)
+              ∗ csp ↦ᵣ WCap RWL Local b_stk e_stk a_stk
+              ∗ (∃ warg0, ca0 ↦ᵣ warg0 ∗ interp W2 C warg0)
+              ∗ (∃ warg1, ca1 ↦ᵣ warg1 ∗ interp W2 C warg1)
+              ∗ ( [∗ map] r↦w ∈ rmap', r ↦ᵣ WInt 0 )
+              ∗ [[ a_stk , a_stk ]] ↦ₐ [[ region_addrs_zeroes a_stk e_stk ]]
+            -∗ WP Seq (Instr Executable) {{ φ }}
+          )
+    )
+    ⊢ WP Seq (Instr Executable) {{ λ v, φ v ∨ ⌜v = FailedV⌝ }}%I.
+  Proof.
+  Admitted.
+
 
 
 
